bugs-found.md
@@ -2,3 +2,4 @@
 
 * https://leanprover.zulipchat.com/#narrow/channel/270676-lean4/topic/Soundness.20bug.3A.20hasLooseBVars.20is.20not.20conservative/near/521286338
 * https://github.com/leanprover/lean4/issues/10475
+* https://github.com/leanprover/lean4/issues/10511
